Definitions/Regions.v
@@ -1,39 +1,49 @@
-(*From stdpp Require Import gmap.*)
+From stdpp Require Import gmap.
 Require Import Ascii.
-Require Import Definitions.Keys.
 
-(* Static Labels *)
-Definition RgnId :=  nat.
-
-(* Program Variables *)
-Definition VarId := ascii.
+Definition RgnVal :=  nat.
+Definition RgnName := ascii.
 
 Inductive Region : bool * bool * bool -> Set :=
-  | Rgn_Const : forall fv bv, RgnId -> Region (true, fv, bv)
-  | Rgn_FVar : forall c bv, VarId -> Region (c, true, bv)
+  | Rgn_Const : forall fv bv, RgnVal -> Region (true, fv, bv)
+  | Rgn_FVar : forall c bv, RgnName -> Region (c, true, bv)
   | Rgn_BVar : forall c fv, nat -> Region (c, fv, true).
 Definition Region_in_Expr := Region (true, true, false).
 Definition Region_in_Type := Region (true, true, true).
 
 
-Module R := FMapAVL.Make (AsciiVars).
-Module RMapP := FMapFacts.Facts R.
-Module RMapProp := FMapFacts.Properties R.
+Definition Rho := gmap RgnName RgnVal.
 
-Definition Rho := R.t RgnId.
-(*Definition Rho := gmap VarId nat.*)
-
-
-Definition find_R (k: Region_in_Expr) (m: Rho) : option RgnId :=
+Definition find_R (k: Region_in_Expr) (m: Rho) : option RgnVal :=
  match k with 
   | Rgn_Const fv bv n => Some n
-  | Rgn_FVar c bv n => R.find (elt := RgnId) n m
+  | Rgn_FVar c bv n =>  m !! n
   | Rgn_BVar c fv n => None                               
  end.
 
-Definition update_R (p: VarId * RgnId) (m : Rho) := R.add (fst p) (snd p) m.
+Definition update_R (p: RgnName * RgnVal) (m : Rho) := <[ (fst p) := (snd p) ]> m.
+
+Definition rho_elem_eq (x y : (RgnName*RgnVal))
+  := eqb (fst x) (fst y) = true /\ Nat.eq (snd x) (snd y).
+
+Lemma rho_elem_eq_dec : forall (k k' : RgnName * RgnVal),
+    { rho_elem_eq k k' } + { ~ rho_elem_eq k k' }.
+Proof.
+  intros. unfold rho_elem_eq, Nat.eq. destruct k as (r, l);
+    destruct k' as (r', l'); subst; simpl.
+  destruct (ascii_dec r r'); destruct (eq_nat_dec l l'). 
+  - left. subst.  split;[apply eqb_refl; reflexivity | reflexivity].
+  - right. intro. contradict n. intuition.
+  - right. intro. destruct H. apply eqb_neq in n.
+    rewrite n in H. contradict H. auto.
+  - right. intro. destruct H. contradict H. subst. contradiction.
+Qed.    
 
 
-(*Export R.
-Export RMapP.
-Export RMapProp.*)
+Open Scope char_scope.
+
+Example rho_as_list : list (RgnName*RgnVal)
+  := ("i"%char, 0)::("j"%char,1)::[].
+
+Example rho_example : gmap RgnName RgnVal
+  := list_to_map rho_as_list.
