Proofs/RegionFacts.v
@@ -1,323 +1,544 @@
+From stdpp Require Import gmap.
+From stdpp Require Import fin_maps.
+From stdpp Require Import list.
+From stdpp Require Import base.
 Require Import Coq.Program.Equality.
 Require Import Coq.Sets.Ensembles.
-Require Import Lia.
 Require Import Definitions.Keys.
 Require Import Definitions.Regions.
 Require Import Definitions.GTypes.
 Require Import Definitions.ComputedActions.
 Require Import Definitions.StaticActions.
 Require Import Coq.FSets.FMapFacts.
+Require Import Ascii.
 
-Lemma R_diff_key_1:
-  forall t a b v v' e,   
+Import Ensembles.
+
+Axiom Rho_SameKey_SameValue:
+  forall (l: list(RgnName*RgnVal)),
+    (forall x y1 y2, (x,y1) ∈ l → (x,y2) ∈ l → y1 = y2).
+
+Lemma rho_NoDup_map_fst:
+  forall (rho : Rho),
+    base.NoDup (map_to_list rho) ->
+    base.NoDup ((map_to_list rho).*1).
+Proof.
+  intros.
+  apply NoDup_fmap_fst; auto.
+  apply Rho_SameKey_SameValue.
+Qed.
+
+
+Lemma find_R_in_list:
+  forall (rho : Rho) (p : RgnName*RgnVal),
+    rho !! p.1 = Some p.2 ->
+    p ∈ map_to_list rho.
+Proof.
+  apply elem_of_map_to_list'.
+Qed.
+  
+
+Lemma G_diff_keys_3 `{Countable K} {A}:
+  forall a b v (m : gmap K A),   
     a <> b ->
-    R.find (elt := t) a (R.add b v e) = Some v' -> 
-    R.find (elt := t) a e = Some v'.
-Proof.
-  intros. 
-  rewrite <- RMapP.find_mapsto_iff in H0. rewrite -> RMapP.add_mapsto_iff in H0.
-  destruct H0; destruct H0; [destruct H | rewrite -> RMapP.find_mapsto_iff in H1]; auto.
-Qed.
-
-Lemma R_diff_key_2:
-  forall t a b v v' e,   
-    b <> a ->
-    R.find (elt := t) a e = Some v' ->
-    R.find (elt := t) a (R.add b v e) = Some v'.
-Proof.
-  intros. 
-  rewrite <- RMapP.find_mapsto_iff. rewrite -> RMapP.add_mapsto_iff.
-  right; split; [exact H | now rewrite RMapP.find_mapsto_iff ].
-Qed.
-
-
-Lemma R_diff_key_3:
-  forall t a b v e,   
-    a <> b ->
-    R.find (elt := t) a (R.add b v e) <> None -> 
-    R.find (elt := t) a e <> None.
-Proof.
-  intros. 
-  rewrite <- RMapP.in_find_iff in H0. rewrite -> RMapP.add_in_iff in H0.
-  intuition. apply RMapP.in_find_iff in H2. contradiction.
-Qed.
-
-
-Lemma find_rho_3:
-  forall x this1 this2 k e t He,
-    R.find (elt:=nat) x {| R.this := R.Raw.Node this1 k e this2 t; R.is_bst := He |} = None ->
-    ~ R.find (elt:=nat) x {| R.this := R.Raw.Node this1 k e this2 t; R.is_bst := He |} 
-    = Some e.
-Proof.
- intros.
- apply RMapP.not_find_in_iff in H.
- contradict H.
- apply RMapP.in_find_iff.
- rewrite H. intro H1. inversion H1.
-Qed.
-
-Lemma not_in_raw_rho:
-  forall x this1 this2 k e  t0 He Hl Hr, 
-    ~ R.In (elt:=nat) x {| R.this := R.Raw.Node this1 k e this2 t0; R.is_bst := He |} ->
-    ~ R.In (elt:=nat) x {| R.this := this1 ; R.is_bst := Hl |}  /\ 
-    ~ R.In (elt:=nat) x {| R.this := this2; R.is_bst := Hr |} /\
-    x <> k /\
-    ~ R.find (elt:=nat) x {| R.this := R.Raw.Node this1 k e this2 t0; R.is_bst := He |} = Some e.
-Proof.
-  intros; repeat split; 
-  try (intro; apply H; apply RMapP.in_find_iff in H0; apply RMapP.in_find_iff; 
-                               contradict H0). 
-  - apply RMapP.not_find_in_iff in H0.
-    apply RMapP.not_find_in_iff. intro. 
-    apply H0. unfold R.In in H1. 
-    unfold R.Raw.In0 in H1.
-    destruct H1.
-    unfold R.In, R.Raw.In0. exists x0.
-    apply  R.Raw.MapsLeft. simpl in H1. 
-    assumption.
-  - apply RMapP.not_find_in_iff in H0. 
-    apply RMapP.not_find_in_iff. intro. 
-    apply H0. unfold R.In in H1. 
-    unfold R.Raw.In0 in H1.
-    destruct H1.
-    unfold R.In, R.Raw.In0. exists x0. simpl. simpl in H1.
-    apply  R.Raw.MapsRight. assumption.
-  - contradict H. rewrite H. clear H. unfold R.In.  
-    econstructor. simpl. econstructor. reflexivity.
-  - apply find_rho_3.
-    apply RMapP.not_find_in_iff.
-    assumption.
-Qed.
-
-Lemma find_rho_1:
-  forall x this1 this2 k e t He Hl,
-    R.find (elt:=nat) x {| R.this := R.Raw.Node this1 k e this2 t; R.is_bst := He |} = None ->
-    R.find (elt:=nat) x {| R.this := this1; R.is_bst := Hl |} = None.
+    (<[ b:=v ]> m) !! a <> None -> 
+    m !! a <> None.
 Proof.
   intros.
-  inversion He; subst.
-  apply RMapP.not_find_in_iff in H.
-  eapply not_in_raw_rho with (Hr:=H6) (Hl:=Hl) in H; auto.
-  destruct H as [HNotIn1 [HNotIn2 [HNotIn3  HNotIn4]]]. 
-  apply RMapP.not_find_in_iff.
-  assumption.
+  contradict H1. apply lookup_insert_None. auto.
 Qed.
 
-Lemma find_rho_2:
-  forall x this1 this2 k e t He Hr,
-    R.find (elt:=nat) x {| R.this := R.Raw.Node this1 k e this2 t; R.is_bst := He |} = None ->
-    R.find (elt:=nat) x {| R.this := this2; R.is_bst := Hr |} = None.
+
+Lemma find_rho_3 `{Countable K} {A}:
+  forall x (m : gmap K A) (e : A),
+    m !! x  = None -> ~ m !! x = Some e.
 Proof.
-  intros.
-  inversion He; subst.
-  apply RMapP.not_find_in_iff in H.
-  eapply not_in_raw_rho with (Hr:=Hr) (Hl:=H4) in H; auto.
-  destruct H as [HNotIn1 [HNotIn2 [HNotIn3  HNotIn4]]]. 
-  apply RMapP.not_find_in_iff.
-  assumption.
+  intros. apply eq_None_not_Some in H0. contradict H0.
+  unfold is_Some. exists e. assumption.
 Qed.
 
-Lemma decompose_find_in_rho:
-  forall x this1 this2 k e v t He Hl Hr, 
-    R.find (elt:=RgnId) x {| R.this := R.Raw.Node this1 k e this2 t; R.is_bst := He |} = Some v ->
-    R.find (elt:=RgnId) x {| R.this := this1; R.is_bst := Hl |} = Some v \/
-    R.find (elt:=RgnId) x {| R.this := this2; R.is_bst := Hr |} = Some v \/
-    e = v.
+ 
+Lemma subst_rgn_aux_comm :
+  forall j1 j2 z1 z2 r,
+    j1 <> j2 ->
+    subst_rgn j1 (Rgn_Const true false z1) (subst_rgn j2 (Rgn_Const true false z2) r) =
+      subst_rgn j2 (Rgn_Const true false z2) (subst_rgn j1 (Rgn_Const true false z1) r).
 Proof.
   intros.
-  apply RMapP.find_mapsto_iff  in H.
-  inversion H; subst.
-  - right. right. reflexivity.
-  - left. apply RMapP.find_mapsto_iff. auto.
-  - right. left.  apply RMapP.find_mapsto_iff. auto.
-Qed. 
+  generalize dependent r.
+  unfold Region_in_Type.
+  dependent induction r; intros; unfold subst_rgn; simpl.
+  - reflexivity.
+  - destruct (AsciiVars.eq_dec j2 r); destruct (AsciiVars.eq_dec j1 r); simpl.
+    + unfold AsciiVars.eq in *; subst. contradiction.
+    + unfold AsciiVars.eq in *; subst.
+      destruct (AsciiVars.eq_dec r r).
+      * reflexivity.
+      * unfold AsciiVars.eq in *; contradiction.
+    + reflexivity.
+    + unfold AsciiVars.eq in *; subst.
+      destruct (AsciiVars.eq_dec j2 r); unfold AsciiVars.eq in *; subst.
+      * contradiction.
+      * reflexivity.
+  - reflexivity.
+Qed.
+
+Lemma subst_sa_aux_comm:
+  forall j1 j2 z1 z2 sa,
+    j1 <> j2 ->
+    subst_sa j1 (Rgn_Const true false z1) (subst_sa j2 (Rgn_Const true false z2) sa) =
+      subst_sa j2 (Rgn_Const true false z2) (subst_sa j1 (Rgn_Const true false z1) sa).
+Proof.
+  intros j1 j2 z1 z2 sa H. induction sa.
+  - generalize dependent r. unfold Region_in_Type. dependent induction r; simpl.
+    + reflexivity.
+    + destruct (AsciiVars.eq_dec j1 r); destruct (AsciiVars.eq_dec j2 r);
+        unfold AsciiVars.eq in *; subst; simpl.
+      * contradiction.
+      * destruct (AsciiVars.eq_dec r r); unfold AsciiVars.eq in *; subst;
+          [reflexivity | contradiction].
+      * destruct (AsciiVars.eq_dec r r); unfold AsciiVars.eq in *; subst;
+          [reflexivity | contradiction].
+      * { destruct (AsciiVars.eq_dec j1 r); destruct (AsciiVars.eq_dec j2 r);
+            unfold AsciiVars.eq in *; subst; simpl.
+          - contradiction.
+          - contradiction.
+          - contradiction.
+          - reflexivity. }
+    + reflexivity.
+  - generalize dependent r. unfold Region_in_Type. dependent induction r; simpl.
+    + reflexivity.
+    + destruct (AsciiVars.eq_dec j1 r); destruct (AsciiVars.eq_dec j2 r);
+        unfold AsciiVars.eq in *; subst; simpl.
+      * contradiction.
+      * destruct (AsciiVars.eq_dec r r); unfold AsciiVars.eq in *; subst;
+          [reflexivity | contradiction].
+      * destruct (AsciiVars.eq_dec r r); unfold AsciiVars.eq in *; subst;
+          [reflexivity | contradiction].
+      * { destruct (AsciiVars.eq_dec j1 r); destruct (AsciiVars.eq_dec j2 r);
+            unfold AsciiVars.eq in *; subst; simpl.
+          - contradiction.
+          - contradiction.
+          - contradiction.
+          - reflexivity. }
+    + reflexivity.
+  - generalize dependent r. unfold Region_in_Type. dependent induction r; simpl.
+    + reflexivity.
+    + destruct (AsciiVars.eq_dec j1 r); destruct (AsciiVars.eq_dec j2 r);
+        unfold AsciiVars.eq in *; subst; simpl.
+      * contradiction.
+      * destruct (AsciiVars.eq_dec r r); unfold AsciiVars.eq in *; subst;
+          [reflexivity | contradiction].
+      * destruct (AsciiVars.eq_dec r r); unfold AsciiVars.eq in *; subst;
+          [reflexivity | contradiction].
+      * { destruct (AsciiVars.eq_dec j1 r); destruct (AsciiVars.eq_dec j2 r);
+            unfold AsciiVars.eq in *; subst; simpl.
+          - contradiction.
+          - contradiction.
+          - contradiction.
+          - reflexivity. }
+    + reflexivity.   
+Qed.
+
+  
+Lemma subst_eps_aux_comm :
+  forall j1 j2 z1 z2 e,
+    j1 <> j2 ->
+    subst_in_eff j1 z1 (subst_in_eff j2 z2 e) =
+      subst_in_eff j2 z2 (subst_in_eff j1 z1 e).
+Proof.
+  intros. unfold subst_in_eff, subst_eps.
+  apply Extensionality_Ensembles.
+  unfold Same_set, Included, Ensembles.In; split; intros x H1. 
+  - destruct H1 as [sa [? ?]].  destruct H0 as [sa' [? ?]].   
+    exists (subst_sa j1 (Rgn_Const true false z1) sa').
+    split. 
+    + exists sa'.
+      split.
+      * auto.
+      * reflexivity.
+    + rewrite <- H1. rewrite <- H2.
+      rewrite subst_sa_aux_comm;[reflexivity | symmetry; assumption].
+  - destruct H1 as [sa [? ?]].  destruct H0 as [sa' [? ?]].   
+    exists (subst_sa j2 (Rgn_Const true false z2) sa').
+    split. 
+    + exists sa'.
+      split.
+      * auto.
+      * reflexivity.
+    + rewrite <- H1. rewrite <- H2.
+      rewrite subst_sa_aux_comm;[reflexivity | assumption].
+Qed.                                        
+
+
+Lemma subst_in_type_fold_foldr:
+  forall (rho : Rho) (ty :Tau),
+    map_fold subst_in_type ty rho =
+      (foldr (uncurry subst_in_type)) ty (map_to_list rho).
+Proof.
+  intros rho tau.
+  apply (map_fold_foldr _ (map_to_list rho)).
+  - solve_proper.
+  - intros j1 j2 z1 z2 y ? ? ?.
+    induction y; try (solve [unfold subst_in_type, subst_type; simpl;reflexivity]).
+    + assert (Hr : forall r u t1 t2,
+                 subst_in_type r u (Ty_Pair t1 t2) =
+                   Ty_Pair (subst_in_type r u t1) (subst_in_type r u t2))
+        by (unfold subst_in_type, subst_type; simpl; f_equal).        
+      do 4 rewrite Hr. f_equal; assumption.
+    + assert (Hr : forall r u rgn ty,
+                 subst_in_type r u (Ty_Ref rgn ty) =
+                   Ty_Ref (subst_rgn r (Rgn_Const true false u) rgn)
+                     (subst_in_type r u ty))
+        by (unfold subst_in_type, subst_type; simpl; f_equal).   
+      do 4 rewrite Hr. f_equal; try (solve [assumption]).
+      rewrite subst_rgn_aux_comm; auto.      
+    + assert (Hr : forall r u aty ceff crty eeff erty,
+                 subst_in_type r u (Ty_Arrow aty ceff crty eeff erty) =
+                   Ty_Arrow (subst_in_type r u aty)
+                     (subst_in_eff r u ceff) (subst_in_type r u crty)
+                     (subst_in_eff r u eeff) (subst_in_type r u erty))
+        by (unfold subst_in_type, subst_type; simpl; f_equal).   
+      do 4 rewrite Hr. f_equal; try (solve [assumption]).
+      rewrite subst_eps_aux_comm; auto.
+      rewrite subst_eps_aux_comm; auto.
+    + assert (Hr : forall r u eff rty,
+                 subst_in_type r u (Ty_ForallRgn eff rty) =
+                   Ty_ForallRgn (subst_in_eff r u eff) (subst_in_type r u rty))
+        by (unfold subst_in_type, subst_type; simpl; f_equal).   
+      do 4 rewrite Hr.
+      f_equal; try (solve [assumption]).
+      rewrite subst_eps_aux_comm; auto.
+  - reflexivity.
+Qed.
+
+Lemma subst_rgn_fold_foldr:
+  forall (rho : Rho) (rt : Region_in_Type),
+    map_fold (fun x r rgn => subst_rgn x (Rgn_Const true false r) rgn) rt rho =
+      (foldr (uncurry(fun x r rgn => subst_rgn x (Rgn_Const true false r) rgn)))
+        rt (map_to_list rho).
+Proof.
+  intros.
+  apply (map_fold_foldr _ (map_to_list rho)).
+  - solve_proper.
+  - intros j1 j2 z1 z2 y ? ? ?.
+    rewrite subst_rgn_aux_comm; auto.
+  - reflexivity.
+Qed.    
+    
 
 Lemma subst_rho_natural :
-  forall rho, subst_rho rho Ty_Natural = Ty_Natural.
+  forall (rho : Rho),
+    subst_rho rho Ty_Natural = Ty_Natural.
 Proof.
-  unfold subst_rho. unfold R.fold. unfold R.Raw.fold.
-  intro rho. destruct rho. simpl. induction this.
+  intros. unfold subst_rho.
+  rewrite subst_in_type_fold_foldr.
+  induction (map_to_list rho); simpl.
   - reflexivity.
-  - inversion is_bst; subst.
-    rewrite IHthis1 by assumption.
-    replace (subst_in_type k e Ty_Natural) with Ty_Natural. 
-    rewrite IHthis2 by assumption.
+  - rewrite IHl.
+    replace (uncurry subst_in_type a Ty_Natural)
+      with (Ty_Natural)
+      by (unfold uncurry; induction a; reflexivity).
     reflexivity.
-    unfold subst_in_type, open_var, close_var.
-    simpl. reflexivity.
 Qed.
 
 Lemma subst_rho_boolean :
   forall rho, subst_rho rho Ty_Boolean = Ty_Boolean.
-Proof.
-  unfold subst_rho. unfold R.fold. unfold R.Raw.fold.
-  intro rho. destruct rho. simpl. induction this.
+Proof.  
+  intros. unfold subst_rho.
+  rewrite subst_in_type_fold_foldr.
+  induction (map_to_list rho); simpl.
   - reflexivity.
-  - inversion is_bst; subst.
-    rewrite IHthis1 by assumption.
-    replace (subst_in_type k e Ty_Boolean) with Ty_Boolean.
-    rewrite IHthis2 by assumption.
+  - rewrite IHl.
+    replace (uncurry subst_in_type a Ty_Boolean)
+      with (Ty_Boolean)
+      by (unfold uncurry; induction a; reflexivity).
     reflexivity.
-    unfold subst_in_type, open_var, close_var.
-    simpl. reflexivity.
 Qed.
 
 Lemma subst_rho_unit :
   forall rho, subst_rho rho Ty_Unit = Ty_Unit.
-Proof.
-  unfold subst_rho. unfold R.fold. unfold R.Raw.fold.
-  intro rho. destruct rho. simpl. induction this.
+Proof.  
+  intros. unfold subst_rho.
+  rewrite subst_in_type_fold_foldr.
+  induction (map_to_list rho); simpl.
   - reflexivity.
-  - inversion is_bst; subst.
-    rewrite IHthis1 by assumption.
-    replace (subst_in_type k e  Ty_Unit) with  Ty_Unit.
-    rewrite IHthis2 by assumption.
+  - rewrite IHl.
+    replace (uncurry subst_in_type a Ty_Unit)
+      with (Ty_Unit)
+      by (unfold uncurry; induction a; reflexivity).
     reflexivity.
-    unfold subst_in_type, open_var, close_var.
-    simpl. reflexivity.
 Qed.
 
 Lemma subst_rho_effect :
   forall rho, subst_rho rho Ty_Effect = Ty_Effect.
 Proof.
-  unfold subst_rho. unfold R.fold. unfold R.Raw.fold.
-  intro rho. destruct rho. simpl. induction this.
+  intros. unfold subst_rho.
+  rewrite subst_in_type_fold_foldr.
+  induction (map_to_list rho); simpl.
   - reflexivity.
-  - inversion is_bst; subst.
-    rewrite IHthis1 by assumption.
-    replace (subst_in_type k e  Ty_Effect) with  Ty_Effect.
-    rewrite IHthis2 by assumption.
+  - rewrite IHl.
+    replace (uncurry subst_in_type a Ty_Effect)
+      with (Ty_Effect)
+      by (unfold uncurry; induction a; reflexivity).
     reflexivity.
-    unfold subst_in_type, open_var, close_var.
-    simpl. reflexivity.
-Qed. 
+Qed.
+
+Lemma fold_subst_rho_free_vars_rgn_not_elem:
+  forall (l: list (RgnName*RgnVal)) (x : RgnName),
+    x ∉ l.*1 ->
+    foldr (uncurry (λ (x0 : RgnName) (r : RgnVal) (rgn : Region_in_Type),
+               subst_rgn x0 (Rgn_Const true false r) rgn))
+      (Rgn_FVar true true x) l =
+      (Rgn_FVar true true x).
+Proof.
+  intros.
+  induction l; simpl.
+   - reflexivity.
+  - rewrite IHl. unfold subst_rgn.
+    destruct a.  simpl. 
+    destruct (AsciiVars.eq_dec r x).
+    + simpl in H. unfold AsciiVars.eq in e; subst. 
+      contradict H. apply elem_of_cons. left. reflexivity.
+    + reflexivity.
+    + apply not_elem_of_cons in H.
+      destruct H. assumption.
+Qed.     
+   
+
+
+Lemma fold_subst_rho_free_vars_rgn_not_elem_2:
+  forall (l: list (RgnName*RgnVal)) (p : (RgnName*RgnVal)),
+    p.1 ∉ dom (list_to_map l : Rho) ->
+    foldr (uncurry (λ (x0 : RgnName) (r : RgnVal) (rgn : Region_in_Type),
+               subst_rgn x0 (Rgn_Const true false r) rgn))
+      (Rgn_FVar true true p.1) l =
+      (Rgn_FVar true true p.1).
+Proof.
+  intros.
+  apply not_elem_of_dom in H.
+  induction l; simpl.
+   - reflexivity.
+   - rewrite IHl.
+     + unfold subst_rgn.  
+       apply not_elem_of_list_to_map in H.
+       apply not_elem_of_cons in H. destruct H. clear H0.
+       destruct a.  simpl in *.
+       destruct (AsciiVars.eq_dec r p.1).
+       * unfold AsciiVars.eq in e.
+         contradict H. auto.
+       * reflexivity.
+     + apply not_elem_of_list_to_map in H.
+       apply not_elem_of_cons in H. destruct H.
+       apply not_elem_of_list_to_map.
+       assumption.
+Qed.     
 
 Lemma fold_subst_rho_free_vars_rgn_aux:
-  forall rho x,
-    R.find (elt:=nat) x rho = None ->
-    fold_subst_rgn rho (Rgn_FVar true true x) =  (Rgn_FVar true true x).
+  forall (rho : Rho) (r : RgnName),
+    rho !! r = None ->
+    fold_subst_rgn rho (Rgn_FVar true true r) = (Rgn_FVar true true r).
 Proof.
-  intros rho. destruct rho. induction this; intros x H.
-  - unfold R.find, R.Raw.find in H. simpl in H.
-    unfold fold_subst_rgn, subst_rgn, R.fold, R.Raw.fold. simpl. 
-    reflexivity.
-  - inversion is_bst; subst.
-    apply RMapP.not_find_in_iff in H. 
-    eapply not_in_raw_rho in H; eauto.
-    destruct H as [HNotIn1 [HNotIn2 [HNotIn3  HNotIn4]]].
-    replace (fold_subst_rgn {| R.this := R.Raw.Node this1 k e this2 t; R.is_bst := is_bst |} 
-                            (Rgn_FVar true true x))
-    with
-    (fold_subst_rgn {| R.this := this2; R.is_bst := H6 |}
-                    (subst_rgn k (Rgn_Const true false e)
-                               (fold_subst_rgn {| R.this := this1; R.is_bst := H4 |} (Rgn_FVar true true x)))
-    ) by (unfold fold_subst_rgn, R.fold, R.Raw.fold in *; reflexivity).
-    apply RMapP.not_find_in_iff in HNotIn1.
-    assert (fold_subst_rgn {| R.this := this1; R.is_bst := H4 |}
-                           (Rgn_FVar true true x) = Rgn_FVar true true x).
-    eapply IHthis1; eauto. rewrite H.
-    apply RMapP.not_find_in_iff in HNotIn2.
-    assert (fold_subst_rgn {| R.this := this2; R.is_bst := H6 |}
-                           (Rgn_FVar true true x) = Rgn_FVar true true x).
-    eapply IHthis2; eauto.
-    unfold subst_rgn. simpl.
-    destruct (AsciiVars.eq_dec k x) as [c | c]; auto.
-    inversion c; subst.
-    contradiction.
+  intros. unfold fold_subst_rgn.
+  rewrite subst_rgn_fold_foldr.
+  apply fold_subst_rho_free_vars_rgn_not_elem.
+  apply not_elem_of_list_to_map.
+  replace (list_to_map (map_to_list rho))
+    with (rho).
+  - assumption.
+  - symmetry. apply list_to_map_to_list.
+Qed.      
+
+Lemma fold_subst_rho_free_vars_rgn_aux_2:
+  forall (l : list (RgnName*RgnVal)) (r : RgnName),
+    r ∉ dom (list_to_map l : Rho) ->
+    fold_subst_rgn (list_to_map l) (Rgn_FVar true true r) = (Rgn_FVar true true r).
+Proof.
+  intros.
+  apply  fold_subst_rho_free_vars_rgn_aux.
+  apply not_elem_of_dom_1 in H.
+  assumption.
 Qed.
+
+
+Lemma subst_rho_rgn_const_aux :
+  forall a c,
+    uncurry (λ (x1 : RgnName) (r : RgnVal) (rgn : Region_in_Type),
+        subst_rgn x1 (Rgn_Const true false r) rgn) a (Rgn_Const true true c) =
+      Rgn_Const true true c.
+Proof.
+  intros. unfold subst_rgn.
+  destruct a. simpl.
+  reflexivity.
+Qed.
+  
 
 Lemma subst_rho_rgn_const :
-  forall rho c, fold_subst_rgn rho (Rgn_Const true true c) = (Rgn_Const true true c).
+  forall rho c,
+    fold_subst_rgn rho (Rgn_Const true true c) = (Rgn_Const true true c).
 Proof.
-  intros rho c.
-  unfold  fold_subst_rgn. unfold R.fold. unfold R.Raw.fold.
-  destruct rho. simpl. induction this.
+  intros.
+  unfold fold_subst_rgn.
+  rewrite subst_rgn_fold_foldr.
+  induction (map_to_list rho); simpl.
   - reflexivity.
-  - inversion is_bst; subst.
-    rewrite IHthis1 by assumption.
-    replace (subst_rgn k (Rgn_Const true false e) (Rgn_Const true true c))
-      with (Rgn_Const true true c).
-    rewrite IHthis2 by assumption.
-    reflexivity.
-    simpl. reflexivity.
-Qed.
+  - rewrite IHl.
+    apply subst_rho_rgn_const_aux.            
+Qed.    
 
 Lemma subst_rho_index :
-  forall rho n, fold_subst_rgn rho (Rgn_BVar true true n) = (Rgn_BVar true true n).
+  forall rho n,
+    fold_subst_rgn rho (Rgn_BVar true true n) = (Rgn_BVar true true n).
 Proof.
-  intros rho n.
-  unfold  fold_subst_rgn. unfold R.fold. unfold R.Raw.fold.
-  destruct rho. simpl. induction this.
+  intros.
+  unfold fold_subst_rgn.
+  rewrite subst_rgn_fold_foldr.
+  induction (map_to_list rho); simpl.
   - reflexivity.
-  - inversion is_bst; subst.
-    rewrite IHthis1 by assumption.
-    replace (subst_rgn k (Rgn_Const true false e) (Rgn_BVar true true n))
-      with (Rgn_BVar true true n).
-    rewrite IHthis2 by assumption.
+  - rewrite IHl. unfold subst_rgn.
+    destruct a. simpl.
     reflexivity.
-    simpl. reflexivity.
-Qed.
-
-Lemma fold_eps_node :
-  forall eff k t e this1 this2
-         (Hl : R.Raw.bst this1)
-         (Hr : R.Raw.bst this2)
-         (is_bst : R.Raw.bst (R.Raw.Node this1 k e this2 t)),
-    fold_subst_eps {| R.this := this2; R.is_bst := Hr |}
-     (subst_eps k (Rgn_Const true false e)
-        (fold_subst_eps {| R.this := this1; R.is_bst := Hl |} eff)) =
-   fold_subst_eps
-     {| R.this := R.Raw.Node this1 k e this2 t; R.is_bst := is_bst |} eff.
-Proof.
-  intros eff k t e this1 this2 Hl Hr is_bst.
-  apply Extensionality_Ensembles;
-  unfold Same_set, Included; split; intros x H; unfold In in *.
-  - unfold fold_subst_eps in *. 
-    destruct H as [sa [[sa' [[sa'' [H1 H2]] H3]] H4]]. 
-    exists sa''. intuition. subst.
-    unfold fold_subst_sa, subst_sa; destruct sa''; f_equal.
-  - unfold fold_subst_eps in *. 
-    destruct H as [sa [H1 H2]]. 
-    exists (subst_sa k (Rgn_Const true false e) (fold_subst_sa {| R.this := this1; R.is_bst := Hl |} sa)).
-    split.
-    + unfold subst_eps.
-      exists (fold_subst_sa {| R.this := this1; R.is_bst := Hl |} sa).
-      intuition. exists sa. intuition.
-    + destruct sa; rewrite <- H2; simpl; f_equal.
 Qed.
 
 Lemma subst_rho_pair : 
   forall rho t1 t2,
     subst_rho rho (Ty_Pair t1 t2) = Ty_Pair (subst_rho rho t1) (subst_rho rho t2).
 Proof.
-  unfold subst_rho.
-  unfold R.fold. unfold R.Raw.fold.
-  intro rho. destruct rho. simpl. induction this; intros t1 t2.
+  intros.
+  unfold subst_rho.  
+  do 3 rewrite subst_in_type_fold_foldr.
+  induction (map_to_list rho); simpl.
   - reflexivity.
-  - assert (Hl: R.Raw.bst this1) by (inversion is_bst; auto).
-    assert (Hr: R.Raw.bst this2) by (inversion is_bst; auto).
-    rewrite IHthis1 by assumption. f_equal. 
-    unfold subst_in_type; simpl.
-    rewrite IHthis2 by assumption. f_equal. 
+  - rewrite IHl; simpl.
+    destruct a.
+    assert (Hr: forall r u t1 t2,
+               (uncurry subst_in_type) (r, u) (Ty_Pair t1 t2) =
+                 Ty_Pair ((uncurry subst_in_type) (r, u) t1)
+                   ((uncurry subst_in_type) (r, u) t2))
+        by (unfold subst_in_type, subst_type; simpl; f_equal).
+    rewrite Hr.
+    f_equal.
 Qed.
 
 
+Definition subst_in_rgn_alt (r : RgnName) (v : RgnVal) (rgn : Region_in_Type)
+  : Region_in_Type
+  := subst_rgn r (Rgn_Const true false v) rgn.
 
-Lemma fold_eps_leaf :
-forall eff is_bst,
-  eff = (fun sa : StaticAction =>
-           exists sa' : StaticAction, eff sa' /\
-                                        fold_subst_sa {| R.this := R.Raw.Leaf RgnId; R.is_bst := is_bst |} sa' = sa).
+Definition fold_subst_rgn_alt (lrho : list(RgnName*RgnVal)) (rt : Region_in_Type)
+(*:= foldr (uncurry (fun x r rgn => subst_rgn x (Rgn_Const true false r) rgn)) rt lrho. *)
+ := foldr (uncurry subst_in_rgn_alt) rt lrho.
+                              
+
+
+Lemma fold_subst_rgn_cons:
+  forall r v l (rt : Region_in_Type),
+    fold_subst_rgn_alt ((r,v) :: l) rt =
+      subst_in_rgn r v (fold_subst_rgn_alt l rt).
 Proof.
- intros eff is_bst.  
- apply Extensionality_Ensembles;
-      unfold Same_set, Included; split; intros x H.
-      * unfold In in *.
-        exists x. intuition. unfold fold_subst_sa. destruct x; unfold fold_subst_rgn, subst_rgn; f_equal.
-      * unfold In in *.  destruct H as [sa [? ?]].
-        assert ( fold_subst_sa {| R.this := R.Raw.Leaf RgnId; R.is_bst := is_bst |} sa = sa)
-          by (unfold fold_subst_sa, fold_subst_rgn, subst_rgn; simpl; destruct sa; subst; f_equal).
-        rewrite H1 in H0. now subst.
+  intros.
+  generalize dependent rt.
+  unfold Region_in_Type. dependent induction rt.
+  - unfold fold_subst_rgn_alt.
+    rewrite foldr_cons; simpl.
+    reflexivity.
+  - unfold fold_subst_rgn_alt.
+    rewrite foldr_cons; simpl.
+    reflexivity.
+  - unfold fold_subst_rgn_alt.
+    rewrite foldr_cons; simpl.
+    reflexivity.
+Qed.    
+
+
+Definition fold_subst_sa_alt (lrho: list (RgnName * RgnVal)) (sa : StaticAction) :=
+  let fn := λ rt,
+      (foldr (uncurry (λ x r rgn, subst_rgn x (Rgn_Const true false r) rgn))) rt lrho
+  in match sa with
+    | SA_Alloc rt => SA_Alloc (fn rt)
+    | SA_Read rt => SA_Read (fn rt)
+    | SA_Write rt => SA_Write (fn rt)
+  end.
+
+Definition head_fold_subst_sa_alt (p: (RgnName * RgnVal)) (sa : StaticAction) :=
+  let fn := λ rt,
+      (uncurry (λ x r rgn, subst_rgn x (Rgn_Const true false r) rgn)) p rt 
+  in match sa with
+    | SA_Alloc rt => SA_Alloc (fn rt)
+    | SA_Read rt => SA_Read (fn rt)
+    | SA_Write rt => SA_Write (fn rt)
+  end.
+
+Lemma fold_subst_sa_cons:
+  forall r rs sa,
+    fold_subst_sa_alt (r :: rs) sa = head_fold_subst_sa_alt r (fold_subst_sa_alt rs sa).
+Proof.
+  intros.
+  unfold fold_subst_sa_alt, head_fold_subst_sa_alt.
+  destruct sa; simpl; f_equal.
+Qed.
+  
+
+Lemma fold_subst_sa_fold_foldr:
+  forall rho sa,
+    fold_subst_sa rho sa = fold_subst_sa_alt (map_to_list rho) sa.
+Proof.
+  intros.
+  unfold fold_subst_sa, fold_subst_sa_alt.
+  induction sa; f_equal; unfold fold_subst_rgn; now rewrite subst_rgn_fold_foldr.
+Qed.
+
+Definition fold_subst_eps_alt (lrho: list (RgnName * RgnVal)) eps :=
+  fun sa => exists sa', eps sa' /\ fold_subst_sa_alt lrho sa' = sa.
+
+Definition fold_subst_eps_alt_head (p: (RgnName * RgnVal)) eps :=
+  fun sa => exists sa', eps sa' /\ head_fold_subst_sa_alt p sa' = sa.
+
+
+Lemma fold_subst_eps_fold_foldr:
+  forall rho eps,
+  fold_subst_eps rho eps = fold_subst_eps_alt (map_to_list rho) eps.
+Proof.
+  intros.
+  unfold fold_subst_eps, fold_subst_eps_alt.
+  apply Extensionality_Ensembles.
+  unfold Same_set, Included, Ensembles.In; split; intros x H.
+  - destruct H as [? [? H2]]. exists x0. split; [assumption|].
+    now rewrite <- fold_subst_sa_fold_foldr.
+  - destruct H as [? [? H2]]. exists x0. split; [assumption|].
+    now rewrite fold_subst_sa_fold_foldr.
+Qed.
+
+
+Lemma fold_subst_eps_cons:
+  forall r rs eps,
+    fold_subst_eps_alt (r :: rs) eps =
+      fold_subst_eps_alt_head r (fold_subst_eps_alt rs eps).
+Proof.
+  intros.
+  apply Extensionality_Ensembles.
+  unfold Same_set, Included, Ensembles.In; split; intros x H.
+  - unfold fold_subst_eps_alt, fold_subst_eps_alt_head in *.
+    destruct x; simpl;
+    destruct H as [sa [H1 H2]].
+    + exists (fold_subst_sa_alt rs sa).
+      split; [exists sa; intuition |].
+      rewrite <- H2. now rewrite fold_subst_sa_cons.
+    + exists (fold_subst_sa_alt rs sa).
+      split; [exists sa; intuition |].
+      rewrite <- H2. now rewrite fold_subst_sa_cons.
+    + exists (fold_subst_sa_alt rs sa).
+      split; [exists sa; intuition |].
+      rewrite <- H2. now rewrite fold_subst_sa_cons.
+  - unfold fold_subst_eps_alt, fold_subst_eps_alt_head in *.
+    destruct x; simpl;
+      destruct H as [sa [[sa' [H1 H2]] H3]].
+    + rewrite <- H2 in H3.
+      exists sa'; split; [assumption | now rewrite fold_subst_sa_cons].
+    + rewrite <- H2 in H3.
+      exists sa'; split; [assumption | now rewrite fold_subst_sa_cons].
+    + rewrite <- H2 in H3.
+      exists sa'; split; [assumption | now rewrite fold_subst_sa_cons].    
 Qed.
 
 
@@ -327,34 +548,68 @@ Lemma subst_rho_arrow :
       Ty_Arrow (subst_rho rho tyr1) (fold_subst_eps rho eff1)
         (subst_rho rho tyr2) (fold_subst_eps rho eff2) (subst_rho rho tyr3) .
 Proof.
-  unfold subst_rho.
-  unfold R.fold. unfold R.Raw.fold.
-  intro rho. destruct rho. simpl. induction this; intros tyr1 eff1 tyr2 eff2 tyr3.
-  - f_equal; unfold fold_subst_eps; apply fold_eps_leaf.
-  - assert (Hl: R.Raw.bst this1) by (inversion is_bst; auto).
-    assert (Hr: R.Raw.bst this2) by (inversion is_bst; auto).
-    rewrite IHthis1 with (is_bst:=Hl) by assumption. f_equal.  
-    unfold subst_in_type; simpl.
-    rewrite IHthis2 with (is_bst:=Hr) by assumption. f_equal.
-    + apply fold_eps_node.
-    + apply fold_eps_node.
-Qed.  
-
-Lemma subst_rho_tyref :
-  forall rho r ty,
-    subst_rho rho (Ty_Ref r ty) = Ty_Ref (fold_subst_rgn rho r) (subst_rho rho ty).
-Proof.
-  unfold subst_rho, fold_subst_rgn. unfold R.fold. unfold R.Raw.fold.
-  intro rho. destruct rho. simpl. induction this; intros r ty.
-  - reflexivity.
-  - inversion is_bst; subst.
-    rewrite IHthis1 by assumption. 
-    unfold subst_in_type, open_var, close_var; simpl.
-    rewrite IHthis2 by assumption.
-    unfold subst_in_type, open_var, close_var. simpl.
-    reflexivity.
-Qed.
-
+  intros.
+  unfold subst_rho. 
+  do 2 rewrite fold_subst_eps_fold_foldr.
+  do 4 rewrite subst_in_type_fold_foldr. 
+  induction (map_to_list rho). simpl.
+  - f_equal.
+    + apply Extensionality_Ensembles.
+      unfold Same_set, Included, Ensembles.In; split; intros sa H1.
+      * exists sa. split; [assumption |].
+        unfold fold_subst_sa_alt.
+        destruct sa; reflexivity.
+      * destruct H1 as [? [? H2]].
+        rewrite <- H2.
+        unfold fold_subst_sa_alt.
+        destruct x; simpl; assumption.
+    + apply Extensionality_Ensembles.
+      unfold Same_set, Included, Ensembles.In; split; intros sa H1.
+      * exists sa. split; [assumption |].
+        unfold fold_subst_sa_alt.
+        destruct sa; reflexivity.
+      * destruct H1 as [? [? H2]].
+        rewrite <- H2.
+        unfold fold_subst_sa_alt.
+        destruct x; simpl; assumption.
+  - do 4 rewrite foldr_cons. 
+    rewrite IHl.
+    assert (Hr : forall r u aty ceff crty eeff erty,
+                 (uncurry subst_in_type) (r, u) (Ty_Arrow aty ceff crty eeff erty) =
+                   Ty_Arrow (uncurry subst_in_type (r, u) aty)
+                     (uncurry subst_in_eff (r, u) ceff) (uncurry subst_in_type (r, u) crty)
+                     (uncurry subst_in_eff (r, u) eeff) (uncurry subst_in_type (r, u) erty))
+        by (unfold subst_in_type, subst_type; simpl; f_equal).   
+    destruct a.
+    rewrite Hr.
+    f_equal.
+    + rewrite fold_subst_eps_cons.
+      apply Extensionality_Ensembles.
+      unfold Same_set, Included, Ensembles.In; split; intros sa H1.
+      * unfold fold_subst_eps_alt_head, fold_subst_eps_alt.
+        unfold subst_in_eff, fold_subst_eps_alt, subst_eps in H1. simpl in H1.
+        destruct H1 as [? [[? [H2 H3]] H4]].
+        exists x.
+        split; [ exists x0; auto | assumption]. 
+      * unfold fold_subst_eps_alt_head, fold_subst_eps_alt.
+        unfold subst_in_eff, fold_subst_eps_alt, subst_eps in H1. simpl in H1.
+        destruct H1 as [? [[? [H2 H3]] H4]].
+        exists x.
+        split; [ exists x0; auto | assumption].
+    + rewrite fold_subst_eps_cons.
+      apply Extensionality_Ensembles.
+      unfold Same_set, Included, Ensembles.In; split; intros sa H1.
+      * unfold fold_subst_eps_alt_head, fold_subst_eps_alt.
+        unfold subst_in_eff, fold_subst_eps_alt, subst_eps in H1. simpl in H1.
+        destruct H1 as [? [[? [H2 H3]] H4]].
+        exists x.
+        split; [ exists x0; auto | assumption]. 
+      * unfold fold_subst_eps_alt_head, fold_subst_eps_alt.
+        unfold subst_in_eff, fold_subst_eps_alt, subst_eps in H1. simpl in H1.
+        destruct H1 as [? [[? [H2 H3]] H4]].
+        exists x.
+        split; [ exists x0; auto | assumption].
+Qed.     
 
 
 Lemma subst_rho_forallrgn  :
@@ -362,100 +617,153 @@ Lemma subst_rho_forallrgn  :
     subst_rho rho (Ty_ForallRgn eff rty) =
       Ty_ForallRgn (fold_subst_eps rho eff) (subst_rho rho rty).
 Proof.
-  unfold subst_rho, fold_subst_eps. unfold R.fold. unfold R.Raw.fold.
-  intro rho. destruct rho. simpl. induction this; intros eff rty.
-  - f_equal; unfold fold_subst_eps; apply fold_eps_leaf.
-  - assert (Hl: R.Raw.bst this1) by (inversion is_bst; auto).
-    assert (Hr: R.Raw.bst this2) by (inversion is_bst; auto).
-    rewrite IHthis1 with (is_bst:=Hl) by assumption. f_equal.  
-    unfold subst_in_type; simpl.
-    rewrite IHthis2 with (is_bst:=Hr) by assumption. f_equal.
-    apply fold_eps_node.
+  intros.
+  unfold subst_rho. 
+  rewrite fold_subst_eps_fold_foldr.
+  do 2 rewrite subst_in_type_fold_foldr. 
+  induction (map_to_list rho); simpl.
+  - f_equal.  apply Extensionality_Ensembles.
+    unfold Same_set, Included, Ensembles.In; split; intros sa H1.
+    + unfold fold_subst_eps_alt.
+      exists sa. split.
+      * assumption.
+      * unfold fold_subst_sa_alt.
+        destruct sa; simpl; reflexivity.
+    + unfold fold_subst_eps_alt in H1.
+      destruct H1 as [? [H2 H3]]. rewrite <- H3.
+      unfold fold_subst_sa_alt.
+      destruct x; simpl; assumption.
+  - rewrite fold_subst_eps_cons. 
+    rewrite IHl.
+    assert (Hr : forall r u eff rty,
+                 (uncurry subst_in_type) (r, u) (Ty_ForallRgn eff rty) =
+                   Ty_ForallRgn (uncurry subst_in_eff (r, u) eff)
+                     (uncurry subst_in_type (r, u) rty))    
+      by (unfold subst_in_type, subst_type; simpl; f_equal).
+    destruct a.
+    rewrite Hr.
+    f_equal.
 Qed.
+    
+ 
+Lemma subst_rho_tyref :
+  forall rho r ty,
+    subst_rho rho (Ty_Ref r ty) = Ty_Ref (fold_subst_rgn rho r) (subst_rho rho ty).
+Proof.
+  intros.
+  unfold subst_rho, fold_subst_rgn.
+  rewrite subst_rgn_fold_foldr. 
+  do 2 rewrite subst_in_type_fold_foldr. 
+  induction (map_to_list rho). simpl.
+  - f_equal.
+  - rewrite foldr_cons.
+    rewrite IHl.
+    assert (Hr : forall x u rgn rty,
+                 (uncurry subst_in_type) (x, u) (Ty_Ref rgn rty) =
+                   Ty_Ref (uncurry  subst_rgn (x, (Rgn_Const true false u)) rgn)
+                     (uncurry subst_in_type (x, u) rty))
+      by (unfold subst_in_type, subst_type; simpl; f_equal).
+    destruct a.
+    rewrite Hr.
+    f_equal.
+Qed.
+
+
 
 Lemma subst_rho_fvar_1:
   forall rho x,
     (exists v, fold_subst_rgn rho (Rgn_FVar true true x) = Rgn_Const true true v) \/ 
     fold_subst_rgn rho (Rgn_FVar true true x) = Rgn_FVar true true x.
 Proof.
-  intro rho. destruct rho. induction this; intros x.
-  - unfold fold_subst_rgn, R.fold, R.Raw.fold; simpl. right. reflexivity.
-  - assert (Hl: R.Raw.bst this1) by (inversion is_bst; auto).
-    assert (Hr: R.Raw.bst this2) by (inversion is_bst; auto).  
-    replace (fold_subst_rgn {| R.this := R.Raw.Node this1 k e this2 t; R.is_bst := is_bst |} (Rgn_FVar true true x))
-    with
-    (fold_subst_rgn {| R.this := this2; R.is_bst := Hr |}
-                    (subst_rgn k (Rgn_Const true false e)
-                               (fold_subst_rgn {| R.this := this1; R.is_bst := Hl |} (Rgn_FVar true true x)))
-    ) by (unfold fold_subst_rgn, R.fold, R.Raw.fold in *; reflexivity).
-    destruct (IHthis1 Hl x).
-    + destruct H as [v ?].
-      left. exists v.
-      rewrite H.  
-      replace (subst_rgn k (Rgn_Const true false e) (Rgn_Const true true v))
-        with (Rgn_Const true true v) by (simpl; reflexivity).
-      apply subst_rho_rgn_const.
-    + rewrite H.
+  intros rho x.
+  unfold fold_subst_rgn.
+  rewrite subst_rgn_fold_foldr.
+  induction (map_to_list); simpl.
+  - right. reflexivity.
+  - destruct IHl. 
+    + left. destruct H. exists x0. rewrite H.
+      apply subst_rho_rgn_const_aux.
+    + rewrite H. 
       unfold subst_rgn.
-      destruct (RMapP.eq_dec k x); subst; simpl.
-      * left. exists e.
-        apply subst_rho_rgn_const.
-      * apply IHthis2.
+      destruct a. simpl. destruct (AsciiVars.eq_dec r x).
+      * left. exists r0. reflexivity.
+      * right. reflexivity. 
+Qed. 
+
+
+Lemma subst_rho_fvar_1_2:
+  forall (l: list(RgnName*RgnVal)) x,
+    (exists v, fold_subst_rgn_alt l (Rgn_FVar true true x) = Rgn_Const true true v) \/ 
+    fold_subst_rgn_alt l (Rgn_FVar true true x) = Rgn_FVar true true x.
+Proof.
+  intros l x.
+  unfold fold_subst_rgn_alt.
+  induction l; simpl.
+  - right. reflexivity.
+  - destruct IHl. 
+    + left. destruct H. exists x0. rewrite H.
+      apply subst_rho_rgn_const_aux.
+    + rewrite H. 
+      unfold subst_rgn.
+      destruct a. simpl. destruct (AsciiVars.eq_dec r x).
+      * left. exists r0. reflexivity.
+      * right. reflexivity. 
 Qed.
 
 Lemma subst_rho_fvar_2:
   forall rho x v,
-   find_R (Rgn_FVar true false x) rho = Some v ->
+   rho !! x = Some v ->
    fold_subst_rgn rho (Rgn_FVar true true x) = Rgn_Const true true v.
 Proof.
-  intro rho.
-  destruct rho. 
-  induction this; intros x v H.
-  - unfold fold_subst_rgn, R.fold, R.Raw.fold; simpl.
-    inversion H.
-  - assert (Hl: R.Raw.bst this1) by (inversion is_bst; auto).
-    assert (Hr: R.Raw.bst this2) by (inversion is_bst; auto). 
-    replace (fold_subst_rgn {| R.this := R.Raw.Node this1 k e this2 t; R.is_bst := is_bst |} 
-                            (Rgn_FVar true true x))
-    with
-    (fold_subst_rgn {| R.this := this2; R.is_bst := Hr |}
-                    (subst_rgn k (Rgn_Const true false e)
-                               (fold_subst_rgn {| R.this := this1; R.is_bst := Hl |} (Rgn_FVar true true x)))
-    ) by (unfold fold_subst_rgn, R.fold, R.Raw.fold in *; reflexivity). 
-    simpl in H. 
-    eapply decompose_find_in_rho in H; eauto.
-    destruct H as [HA | [HB | HC]].  
-    + assert (H' : fold_subst_rgn {| R.this := this1; R.is_bst := Hl |}
-                                 (Rgn_FVar true true x) = Rgn_Const true true v)
-       by (apply IHthis1; simpl; assumption).    
-      rewrite H'. simpl. rewrite subst_rho_rgn_const. reflexivity.
-    + assert (H'' : fold_subst_rgn {| R.this := this2; R.is_bst := Hr |}
-                                 (Rgn_FVar true true x) = Rgn_Const true true v)
-          by (apply IHthis2; simpl; assumption).
-      rewrite<- H''. unfold subst_rgn. simpl.
-      admit.
-    + subst.
-      replace (subst_rgn k (Rgn_Const true false v)
-                 (fold_subst_rgn {| R.this := this1; R.is_bst := Hl |}
-                    (Rgn_FVar true true x))) with (Rgn_Const true true v).
-      admit.
-Admitted.
+  intros rho x v HSome.
+  assert ((x,v) ∈ map_to_list rho) by (apply elem_of_map_to_list'; auto).
+  unfold fold_subst_rgn. 
+  rewrite subst_rgn_fold_foldr.   
+  assert (H' : base.NoDup (map_to_list rho)) by (apply NoDup_map_to_list).
+  assert (HNoDup: base.NoDup ((map_to_list rho).*1))
+    by (now apply rho_NoDup_map_fst).    
+  clear H'. 
+  induction (map_to_list rho); simpl.  
+  - contradict H.
+    apply not_elem_of_nil. 
+  - apply elem_of_cons in H. 
+    destruct H.
+    + clear IHl. 
+      subst.  simpl. 
+      replace ((foldr (uncurry
+          (λ (x0 : RgnName) (r : RgnVal) (rgn : Region_in_Type),
+            subst_rgn x0 (Rgn_Const true false r) rgn)) (Rgn_FVar true true x) l))
+        with (Rgn_FVar true true x).
+      * simpl. destruct (AsciiVars.eq_dec x x). 
+        reflexivity. unfold AsciiVars.eq in n. contradiction.
+      * { apply list.NoDup_cons in HNoDup.
+          rewrite fold_subst_rho_free_vars_rgn_not_elem.
+          - reflexivity. 
+          - destruct HNoDup.
+            assumption. }
+    + rewrite IHl.
+      * destruct a. unfold subst_rgn. simpl. reflexivity.
+      * assumption.
+      * apply list.NoDup_cons in HNoDup.
+        destruct HNoDup. assumption.
+Qed.
+
 
 Lemma subst_rho_free_vars_rgn:
  forall rho x r,
-   R.find (elt:=RgnId) x rho = None ->
+   rho !! x = None ->
    not_set_elem (free_rgn_vars_in_rgn (fold_subst_rgn rho r)) x ->
    not_set_elem (free_rgn_vars_in_rgn r) x.
 Proof.
   intros rho x r HFind HNotElem.
   unfold Region_in_Type in r. dependent induction r. 
   - rewrite subst_rho_rgn_const in HNotElem. assumption.
-  - assert ((exists v', fold_subst_rgn rho (Rgn_FVar true true v) =  
+  - assert ((exists v', fold_subst_rgn rho (Rgn_FVar true true r) =  
                          Rgn_Const true true v') \/ 
-            fold_subst_rgn rho (Rgn_FVar true true v) = Rgn_FVar true true v) 
+            fold_subst_rgn rho (Rgn_FVar true true r) = Rgn_FVar true true r) 
       by (apply subst_rho_fvar_1).
-    destruct (subst_rho_fvar_1 rho v) as [[v' H0] | H0]; simpl in *.
-    + destruct (AsciiVars.eq_dec v x) as [c | c]; auto.
+    destruct (subst_rho_fvar_1 rho r) as [[v' H0] | H0]; simpl in *.
+    + destruct (AsciiVars.eq_dec r x) as [c | c]; auto.
       * inversion c; subst. intro.
         rewrite fold_subst_rho_free_vars_rgn_aux in H0; auto.
         inversion H0.
@@ -466,8 +774,7 @@ Proof.
   - rewrite subst_rho_index in HNotElem. 
     assumption.
 Qed.
-
-
+    
 
 Lemma TcRhoIncludedNoFreeVarsRgn_aux_fold:
   forall rho r x,
@@ -477,9 +784,9 @@ Proof.
   intros. 
   unfold Region_in_Type in r; dependent induction r.
   - rewrite subst_rho_rgn_const in H. assumption.
-  - assert ((exists v', fold_subst_rgn rho (Rgn_FVar true true v)
+  - assert ((exists v', fold_subst_rgn rho (Rgn_FVar true true r)
                         = Rgn_Const true true v') \/ 
-            fold_subst_rgn rho (Rgn_FVar true true v) = Rgn_FVar true true v) 
+            fold_subst_rgn rho (Rgn_FVar true true r) = Rgn_FVar true true r) 
       by (apply subst_rho_fvar_1).
     destruct H0. 
     + destruct H0. rewrite H0 in H. 
@@ -490,27 +797,257 @@ Proof.
 Qed.
 
 
+Lemma subst_rho_rgn_const_2 :
+  forall l c,
+    fold_subst_rgn_alt l (Rgn_Const true true c) = (Rgn_Const true true c).
+Proof.
+  intros.
+  unfold fold_subst_rgn_alt.
+  induction l; simpl.
+  - reflexivity.
+  - rewrite IHl.
+    apply subst_rho_rgn_const_aux.            
+Qed.
+
+Lemma subst_rho_index_2 :
+  forall l n,
+    fold_subst_rgn_alt l (Rgn_BVar true true n) = (Rgn_BVar true true n).
+Proof.
+  intros.
+  unfold fold_subst_rgn_alt.
+  induction l; simpl.
+  - reflexivity.
+  - rewrite IHl. unfold subst_rgn.
+    destruct a. simpl.
+    reflexivity.
+Qed.
+
+Lemma TcRhoIncludedNoFreeVarsRgn_aux_fold_2:
+  forall (l : list (RgnName*RgnVal)) r x,
+    free_rgn_vars_in_rgn (fold_subst_rgn_alt l r) x ->
+    free_rgn_vars_in_rgn r x.
+Proof.
+  intros. 
+  unfold Region_in_Type in r; dependent induction r.
+  - rewrite subst_rho_rgn_const_2 in H. assumption.
+  - assert ((exists v', fold_subst_rgn_alt l (Rgn_FVar true true r)
+                        = Rgn_Const true true v') \/ 
+            fold_subst_rgn_alt l (Rgn_FVar true true r) = Rgn_FVar true true r) 
+      by (apply subst_rho_fvar_1_2).
+    destruct H0. 
+    + destruct H0. rewrite H0 in H. 
+      unfold free_rgn_vars_in_rgn in H. inversion H.
+    + rewrite H0 in H.
+      assumption.
+  - rewrite subst_rho_index_2 in H. assumption.
+Qed.
+
+
 Lemma TcRhoIncludedNoFreeVarsSa_aux_fold:
   forall rho sa x,
-    free_rgn_vars_in_sa (fold_subst_sa rho sa) x ->
+    free_rgn_vars_in_sa (fold_subst_sa_alt rho sa) x ->
     free_rgn_vars_in_sa sa x.
 Proof.
   intros. 
-  induction sa; unfold free_rgn_vars_in_sa, fold_subst_sa in *;
-  eapply TcRhoIncludedNoFreeVarsRgn_aux_fold; eauto. 
+  induction sa; unfold free_rgn_vars_in_sa, fold_subst_sa_alt in *;
+    eapply TcRhoIncludedNoFreeVarsRgn_aux_fold_2; eauto. 
 Qed.
  
 Lemma TcRhoIncludedNoFreeVarsEps_aux_fold:
   forall rho e x,
-    free_rgn_vars_in_eps (fold_subst_eps rho e) x ->
+    free_rgn_vars_in_eps (fold_subst_eps_alt rho e) x ->
     free_rgn_vars_in_eps e x.
 Proof.
-  intros. unfold  free_rgn_vars_in_eps, fold_subst_eps in *.
+  intros. unfold  free_rgn_vars_in_eps, fold_subst_eps_alt in *.
   destruct H as [sa [[sa' [H1 H2]] H3]].
   exists sa'. intuition.
   rewrite <- H2 in H3.
   eapply TcRhoIncludedNoFreeVarsSa_aux_fold; eauto.
 Qed.
+
+
+Lemma TcRhoIncludedNoFreeVarsSa_aux_fold_2:
+  forall a sa x,
+    free_rgn_vars_in_sa (head_fold_subst_sa_alt a sa) x ->
+    free_rgn_vars_in_sa sa x.
+Proof.
+  intros.
+  induction sa. unfold free_rgn_vars_in_sa in *.
+  - unfold head_fold_subst_sa_alt in H.
+    apply TcRhoIncludedNoFreeVarsRgn_aux_fold_2 with (l:= cons a nil).
+    now assumption.
+  - unfold head_fold_subst_sa_alt in H.
+    apply TcRhoIncludedNoFreeVarsRgn_aux_fold_2 with (l:= cons a nil).
+    now assumption.
+  - unfold head_fold_subst_sa_alt in H.
+    apply TcRhoIncludedNoFreeVarsRgn_aux_fold_2 with (l:= cons a nil).
+    now assumption.
+Qed. 
+
+
+Lemma TcRhoIncludedNoFreeVarsEps_aux_fold_1:
+  forall (a : (RgnName * RgnVal)) e (x: RgnName),
+    free_rgn_vars_in_eps (fold_subst_eps_alt_head a e) x ->
+    free_rgn_vars_in_eps e x.
+Proof.
+  intros.
+  intros. unfold  free_rgn_vars_in_eps, fold_subst_eps in *.
+  destruct H as [sa [[sa' [H1 H2]] H3]].
+  exists sa'. intuition.
+  rewrite <- H2 in H3.
+  eapply TcRhoIncludedNoFreeVarsSa_aux_fold_2; eauto.
+Qed.
+
+
+Lemma subst_rgn_fold_foldr_3:
+  forall k v (l : list (RgnName*RgnVal)) (rt : Region_in_Type),
+    base.NoDup l.*1 ->
+    (list_to_map l : Rho) !! k = None ->
+    map_fold (fun x r rgn => subst_rgn x (Rgn_Const true false r) rgn)
+      rt (<[k:=v]> (list_to_map l : Rho)) =
+      (foldr (uncurry(fun x r rgn => subst_rgn x (Rgn_Const true false r) rgn)))
+        rt ((k, v)::l).
+Proof.
+  intros.
+  apply (map_fold_foldr _ ((k, v)::l)).
+  - solve_proper.
+  - intros j1 j2 z1 z2 y ? ? ?.
+    rewrite subst_rgn_aux_comm; auto.
+  -  assert (map_to_list (<[k:=v]> (list_to_map l)) ≡ₚ
+              (k, v) :: map_to_list(list_to_map l))
+       by (apply map_to_list_insert; assumption).
+     rewrite H1.
+     rewrite map_to_list_to_map.
+     + reflexivity.
+     + assumption.
+Qed.
+
+
+Lemma fold_subst_SA_Alloc_head_insert:
+  forall k v (l: list (RgnName*RgnVal)) (r: Region_in_Type),
+    (list_to_map l : Rho) !! k = None ->
+    base.NoDup l.*1 ->
+    head_fold_subst_sa_alt (k, v) (fold_subst_sa_alt l (SA_Alloc r)) =
+      SA_Alloc (fold_subst_rgn (<[k:=v]> (list_to_map l)) r).
+Proof.
+  intros.
+  unfold fold_subst_rgn.  
+  unfold Region_in_Type in r; dependent induction r. simpl.
+  - f_equal. rewrite subst_rgn_fold_foldr_3.
+    + simpl. reflexivity.
+    + assumption.
+    + assumption.
+  - f_equal. rewrite subst_rgn_fold_foldr_3.
+    + simpl. reflexivity.
+    + assumption.
+    + assumption.
+  - f_equal. rewrite subst_rgn_fold_foldr_3.
+    + simpl. reflexivity.
+    + assumption.
+    + assumption.        
+Qed.
+
+Lemma fold_subst_SA_Read_head_insert:
+  forall k v l (r: Region_in_Type),
+    (list_to_map l : Rho) !! k = None ->
+    base.NoDup l.*1 ->
+    head_fold_subst_sa_alt (k,v) (fold_subst_sa_alt l (SA_Read r)) =
+      SA_Read (fold_subst_rgn (<[k:=v]> (list_to_map l)) r).
+Proof.
+  intros.
+  unfold fold_subst_rgn.  
+  unfold Region_in_Type in r; dependent induction r. simpl.
+  - f_equal. rewrite subst_rgn_fold_foldr_3.
+    + simpl. reflexivity.
+    + assumption.
+    + assumption.
+  - f_equal. rewrite subst_rgn_fold_foldr_3.
+    + simpl. reflexivity.
+    + assumption.
+    + assumption.
+  - f_equal. rewrite subst_rgn_fold_foldr_3.
+    + simpl. reflexivity.
+    + assumption.
+    + assumption.
+Qed.
+
+Lemma fold_subst_SA_Write_head_insert:
+  forall k v l (r: Region_in_Type),
+    (list_to_map l : Rho) !! k = None ->
+    base.NoDup l.*1 ->
+    head_fold_subst_sa_alt (k,v) (fold_subst_sa_alt l (SA_Write r)) =
+      SA_Write (fold_subst_rgn (<[k:=v]> (list_to_map l)) r).
+Proof.
+  intros.
+  unfold fold_subst_rgn.  
+  unfold Region_in_Type in r; dependent induction r. simpl.
+  - f_equal. rewrite subst_rgn_fold_foldr_3.
+    + simpl. reflexivity.
+    + assumption.
+    + assumption.
+  - f_equal. rewrite subst_rgn_fold_foldr_3.
+    + simpl. reflexivity.
+    + assumption.
+    + assumption.
+  - f_equal. rewrite subst_rgn_fold_foldr_3.
+    + simpl. reflexivity.
+    + assumption.
+    + assumption.
+Qed.
+
+
+Lemma fold_subst_sa_map_to_list:
+  forall a (l : list (RgnName*RgnVal)) sa,
+    (list_to_map l : Rho) !! a.1 = None ->
+    base.NoDup l.*1 ->
+    fold_subst_sa_alt (a :: l) sa = fold_subst_sa (<[a.1:=a.2]> (list_to_map l)) sa.
+Proof.
+  intros.
+  rewrite fold_subst_sa_cons.
+  unfold fold_subst_sa, fold_subst_rgn_alt.
+  destruct sa; destruct a as [k v].
+  - apply fold_subst_SA_Alloc_head_insert; auto.
+  - apply fold_subst_SA_Read_head_insert; auto.
+  - apply fold_subst_SA_Write_head_insert; auto.
+Qed.
+
+
+
+Lemma free_rgn_vars_in_eps_map_to_list_2:
+  forall (l : list (RgnName*RgnVal)) e x,
+    base.NoDup l.*1 ->
+    free_rgn_vars_in_eps (fold_subst_eps (list_to_map l) e) x ->
+    free_rgn_vars_in_eps (fold_subst_eps_alt l e) x.
+Proof.
+  intros l e x HNoDup H.
+  induction l; simpl in H;
+    unfold fold_subst_eps_alt;
+    unfold fold_subst_eps in H;
+    destruct H as [sa [[sa' [H1 H2]] H3]];
+    unfold free_rgn_vars_in_eps.
+  - exists sa. split; [exists sa'; intuition | assumption].
+  - apply list.NoDup_cons in HNoDup. destruct HNoDup.
+    exists sa. split.
+    + exists sa'. intuition.
+      rewrite <- H2. 
+      apply fold_subst_sa_map_to_list.
+      apply not_elem_of_list_to_map_1.
+      * assumption.
+      * assumption. 
+    + assumption.      
+Qed.
+
+Lemma free_rgn_vars_in_eps_map_to_list:
+  forall (rho: Rho) e x,
+    free_rgn_vars_in_eps (fold_subst_eps rho e) x ->
+    free_rgn_vars_in_eps (fold_subst_eps_alt (map_to_list rho) e) x.
+Proof.
+  intros.
+  replace (fold_subst_eps rho e) with (fold_subst_eps_alt (map_to_list rho) e) in H.
+  - assumption.
+  - symmetry. apply fold_subst_eps_fold_foldr.
+Qed.
+
 
 Lemma TcRhoIncludedNoFreeVarsSa:
   forall k rc r x,
@@ -522,11 +1059,12 @@ Proof.
   dependent induction r;
   unfold free_rgn_vars_in_rgn, subst_rgn in *; simpl.
   - inversion H.
-  - destruct (RMapProp.F.eq_dec k v); subst; simpl in *.
+  - destruct (AsciiVars.eq_dec k r); subst; simpl in *.
     + inversion H.
     + assumption.
   - inversion H.
 Qed.
+
 
 Lemma TcRhoIncludedNoFreeVarsRgn:
   forall k rc sa x,
@@ -576,7 +1114,7 @@ Proof.
   unfold Region_in_Type in r; dependent induction r; simpl; 
   try (solve [ intro; contradict H | 
                intro; unfold free_rgn_vars_in_rgn in H;
-               destruct (RMapProp.F.eq_dec x v); subst; 
+               destruct (AsciiVars.eq_dec x r); subst; 
                [inversion H | inversion H; symmetry in H0; contradiction] ]).
 Qed.
 
@@ -618,26 +1156,26 @@ Proof.
   dependent induction r0; intros.
   - rewrite subst_rho_rgn_const in H.
     simpl in H. contradiction.
-  - destruct (AsciiVars.eq_dec x v) as [c | c].
+  - destruct (AsciiVars.eq_dec x r) as [c | c].
     + inversion c; subst.   
       inversion HRho; subst.   
       contradict H.
-      destruct (subst_rho_fvar_1 rho v) as [[v' H0] | H0]. 
+      destruct (subst_rho_fvar_1 rho r) as [[v' H0] | H0]. 
       * rewrite H0. simpl. intro. contradiction.
       * rewrite H0. simpl. intro. 
         unfold set_elem, In in H1.
-        destruct H1 with (r:=v). 
+        destruct H1 with (r:=r). 
         { apply H3 in HInc.
           - apply NotNoneIsSome in HInc.
             destruct HInc.
-            apply subst_rho_fvar_2 in H4.
+            apply subst_rho_fvar_2 in H4. 
             rewrite H4 in H0. 
             inversion H0.
           - apply Union_introl. simpl. auto. }
    + unfold AsciiVars.eq in c; subst.   
      inversion HRho; subst.
      contradict H.
-     destruct (subst_rho_fvar_1 rho v) as [[v' H0] | H0].
+     destruct (subst_rho_fvar_1 rho r) as [[v' H0] | H0].
      * rewrite H0. simpl. intro. contradiction.
      * rewrite H0. simpl. intro. inversion H. auto.
   - rewrite subst_rho_index in H.
@@ -645,93 +1183,225 @@ Proof.
 Qed.
 
 
-Module RProofs := R.Raw.Proofs.
-Lemma FindIfLowerThan:
-  forall x this1 this2 k e t is_bst H,
-    R.find (elt:=RgnId) x
-        {| R.this := R.Raw.Node this1 k e this2 t; R.is_bst := is_bst |} <> None ->
-    AsciiVars.lt x k ->
-    R.find (elt:=RgnId) x {| R.this := this1; R.is_bst := H |} <> None.
+Lemma not_free_vars_in_head_after_subst:
+  forall x v sa,
+    ~free_rgn_vars_in_sa (head_fold_subst_sa_alt (x, v) sa) x.
 Proof.
-  intros x this1 this2 k e t is_bst H H1 H2.
-  inversion is_bst; subst.
-  apply RProofs.find_in in H1.  
-  inversion H1; subst. 
-  - unfold AsciiVars.lt in H2; lia.
-  - apply RProofs.in_find.
-    + inversion is_bst; subst.
-      assumption.
-    + assumption.
-  - apply RProofs.in_find.
-    + assumption.
-    + eapply RProofs.gt_tree_trans in H2; eauto.
-      assert (~ R.Raw.In x this2) by (apply RProofs.gt_tree_not_in in H2; auto).
-      contradiction.
-Qed.    
+  intros.
+  unfold head_fold_subst_sa_alt. destruct sa;
+   unfold Region_in_Type in r;
+  dependent induction r;
+    unfold free_rgn_vars_in_rgn, subst_rgn in *; simpl;
+    try( solve[intro; inversion H]).
+  - destruct (AsciiVars.eq_dec x r).
+    + unfold AsciiVars.eq in e; subst.
+      unfold free_rgn_vars_in_rgn.
+      intro. inversion H.
+    + unfold free_rgn_vars_in_rgn.
+      intro. inversion H. unfold AsciiVars.eq in n; subst. contradiction.
+  - destruct (AsciiVars.eq_dec x r).
+    + unfold AsciiVars.eq in e; subst.
+      unfold free_rgn_vars_in_rgn.
+      intro. inversion H.
+    + unfold free_rgn_vars_in_rgn.
+      intro. inversion H. unfold AsciiVars.eq in n; subst. contradiction.
+  - destruct (AsciiVars.eq_dec x r).
+    + unfold AsciiVars.eq in e; subst.
+      unfold free_rgn_vars_in_rgn.
+      intro. inversion H.
+    + unfold free_rgn_vars_in_rgn.
+      intro. inversion H. unfold AsciiVars.eq in n; subst. contradiction.
+Qed. 
 
-Lemma FindIfGreaterThan:
-  forall x this1 this2 k e t is_bst H,
-    R.find (elt:=RgnId) x
-        {| R.this := R.Raw.Node this1 k e this2 t; R.is_bst := is_bst |} <> None ->
-    AsciiVars.lt k x ->
-    R.find (elt:=RgnId) x {| R.this := this2; R.is_bst := H |} <> None.
+Lemma not_free_vars_in_head_after_subst_2:
+  forall r x v sa,
+    r <> x ->
+    free_rgn_vars_in_sa (head_fold_subst_sa_alt (r, v) sa) x ->
+    free_rgn_vars_in_sa sa x.
 Proof.
-  intros x this1 this2 k e t is_bst H H1 H2.
-  inversion is_bst; subst.
-  apply RProofs.find_in in H1.  
-  inversion H1; subst. 
-  - unfold AsciiVars.lt in H2; lia.
- - apply RProofs.in_find.
-    + assumption.
-    + eapply RProofs.lt_tree_trans in H2; eauto.
-      assert (~ R.Raw.In x this1) by (apply RProofs.lt_tree_not_in in H2; auto).
-      contradiction.
-  - apply RProofs.in_find.
-    + inversion is_bst; subst.
-      assumption.
-    + assumption.
+  intros. unfold free_rgn_vars_in_sa in *.
+  unfold head_fold_subst_sa_alt in *. 
+  unfold fold_subst_sa_alt in *.
+  destruct sa;
+  unfold Region_in_Type in r0;
+  dependent induction r0;
+  unfold free_rgn_vars_in_rgn, subst_rgn in *;
+    simpl in *; try (solve
+                       [assumption |
+                         destruct (AsciiVars.eq_dec r r0); [inversion H0 |
+                                                             assumption]]).
 Qed.
 
+Lemma TcRhoIncludedNoFreeVarsSa_aux_fold_3:
+  forall l sa a x,
+    free_rgn_vars_in_sa (head_fold_subst_sa_alt a (fold_subst_sa_alt l sa)) x ->
+    free_rgn_vars_in_sa sa x.
+Proof.
+  intros.
+  apply TcRhoIncludedNoFreeVarsSa_aux_fold with (rho:=l).
+  destruct a as [r v].
+  destruct (ascii_dec r x); subst; simpl in *.
+  - contradict H. apply not_free_vars_in_head_after_subst.
+  - eapply not_free_vars_in_head_after_subst_2; eauto.
+Qed.  
+
+Lemma subst_rgn_not_elem_1:
+  forall r v x,
+    x ≠ r ->
+    uncurry (λ (x0 : RgnName) (r0 : RgnVal) (rgn : Region_in_Type),
+        subst_rgn x0 (Rgn_Const true false r0) rgn)
+      (r, v) (Rgn_FVar true true x) = (Rgn_FVar true true x).
+Proof.
+  intros.
+  unfold subst_rgn. simpl.
+  destruct (AsciiVars.eq_dec r x); unfold AsciiVars.eq in *; subst.
+  - contradiction.
+  - reflexivity.
+Qed.
+
+Lemma subst_rgn_not_elem_2:
+  forall r v n,
+    uncurry
+      (λ (x0 : RgnName) (r0 : RgnVal) (rgn : Region_in_Type),
+        subst_rgn x0 (Rgn_Const true false r0) rgn)
+      (r, v) (Rgn_BVar true true n) = (Rgn_BVar true true n).
+Proof.
+  intros.
+  unfold subst_rgn. simpl.
+  reflexivity.
+Qed.
+
+                                                    
+Lemma not_free_vars_compose_head_sa_fold:
+  forall r v sa x,
+    free_rgn_vars_in_sa sa x ->
+    x ≠ r ->
+    free_rgn_vars_in_sa (head_fold_subst_sa_alt (r, v) sa) x.
+Proof.
+  intros. unfold free_rgn_vars_in_sa in *.
+  unfold head_fold_subst_sa_alt in *. 
+  unfold fold_subst_sa_alt in *.
+  destruct sa;
+  unfold Region_in_Type in r0;
+  dependent induction r0;
+    unfold free_rgn_vars_in_rgn. try (solve [unfold subst_rgn in *; assumption]).
+  - inversion H; subst.
+    replace (uncurry
+      (λ (x0 : RgnName) (r0 : RgnVal) (rgn : Region_in_Type),
+        subst_rgn x0 (Rgn_Const true false r0) rgn) (r, v) (Rgn_FVar true true x))
+      with (Rgn_FVar true true x).
+    + apply In_singleton.
+    + symmetry; apply subst_rgn_not_elem_1; auto.
+  - replace ( uncurry
+      (λ (x0 : RgnName) (r0 : RgnVal) (rgn : Region_in_Type),
+        subst_rgn x0 (Rgn_Const true false r0) rgn) (r, v) (Rgn_BVar true true n))
+      with (Rgn_BVar true true n).
+    + inversion H.
+    + unfold subst_rgn. simpl.
+      reflexivity.
+  - replace (uncurry
+      (λ (x0 : RgnName) (r1 : RgnVal) (rgn : Region_in_Type),
+        subst_rgn x0 (Rgn_Const true false r1) rgn) (r, v) (Rgn_Const true true r0))
+              with ((Rgn_Const true true r0)).
+    + inversion H.
+    + unfold subst_rgn. simpl.
+      reflexivity.
+  - inversion H; subst.
+    replace (uncurry
+      (λ (x0 : RgnName) (r0 : RgnVal) (rgn : Region_in_Type),
+        subst_rgn x0 (Rgn_Const true false r0) rgn) (r, v) (Rgn_FVar true true x))
+      with (Rgn_FVar true true x).
+    + apply In_singleton.
+    + symmetry; apply subst_rgn_not_elem_1; auto.
+  - replace ( uncurry
+      (λ (x0 : RgnName) (r0 : RgnVal) (rgn : Region_in_Type),
+        subst_rgn x0 (Rgn_Const true false r0) rgn) (r, v) (Rgn_BVar true true n))
+      with (Rgn_BVar true true n).
+    + inversion H.
+    + unfold subst_rgn. simpl.
+      reflexivity.
+  - replace (uncurry
+      (λ (x0 : RgnName) (r1 : RgnVal) (rgn : Region_in_Type),
+        subst_rgn x0 (Rgn_Const true false r1) rgn) (r, v) (Rgn_Const true true r0))
+              with ((Rgn_Const true true r0)).
+    + inversion H.
+    + unfold subst_rgn. simpl.
+      reflexivity.
+  - inversion H; subst.
+    replace (uncurry
+      (λ (x0 : RgnName) (r0 : RgnVal) (rgn : Region_in_Type),
+        subst_rgn x0 (Rgn_Const true false r0) rgn) (r, v) (Rgn_FVar true true x))
+      with (Rgn_FVar true true x).
+    + apply In_singleton.
+    + symmetry; apply subst_rgn_not_elem_1; auto.
+  - replace ( uncurry
+      (λ (x0 : RgnName) (r0 : RgnVal) (rgn : Region_in_Type),
+        subst_rgn x0 (Rgn_Const true false r0) rgn) (r, v) (Rgn_BVar true true n))
+      with (Rgn_BVar true true n).
+    + inversion H.
+    + unfold subst_rgn. simpl.
+      reflexivity.
+Qed.      
+     
+   
+
+Lemma not_free_vars_compose_head_eps_fold:
+  forall a l e x,
+    ~ (free_rgn_vars_in_eps (fold_subst_eps_alt_head a e) x /\
+         free_rgn_vars_in_eps (fold_subst_eps_alt l e) x) ->
+    ~free_rgn_vars_in_eps (fold_subst_eps_alt_head a (fold_subst_eps_alt l e)) x.    
+Proof.
+  intros. intro. apply H. split. clear H. 
+  - unfold free_rgn_vars_in_eps in H0. 
+    destruct H0 as [sa [H1 H2]].
+    unfold fold_subst_eps_alt_head in H1.
+    destruct H1 as [sa' [Ha Hb]].
+    unfold fold_subst_eps_alt in Ha.
+    destruct Ha as [sa'' [Hf Hg]].
+    destruct a as [r v].
+    destruct (ascii_dec x r).
+    + subst. contradict H2.
+      apply not_free_vars_in_head_after_subst.
+    + subst.
+      unfold free_rgn_vars_in_eps. unfold fold_subst_eps_alt_head.
+      exists (head_fold_subst_sa_alt (r, v) sa'').
+      split.
+      * unfold fold_subst_eps_alt_head.
+        exists sa''. intuition.
+      * subst.    
+        apply not_free_vars_in_head_after_subst_2 in H2; auto.
+        apply TcRhoIncludedNoFreeVarsSa_aux_fold in H2.
+        apply not_free_vars_compose_head_sa_fold; auto.
+  - apply TcRhoIncludedNoFreeVarsEps_aux_fold_1 in H0.
+    assumption.
+Qed.
+
+
 Lemma TcRhoIncludedNoFreeVarsEps_find:
-  forall rho x,
-    R.find x rho <> None ->
-    forall e,
-      ~ (free_rgn_vars_in_eps (fold_subst_eps rho e)) x.
-Proof. 
-  intros rho. destruct rho. induction this; intros x H e'.
-  - unfold fold_subst_eps.
-    replace (fun sa : StaticAction =>
-               exists sa' : StaticAction,
-                 e' sa' /\
-                 fold_subst_sa {| R.this := R.Raw.Leaf nat; R.is_bst := is_bst |} sa' =
-                 sa)
-    with e' by (rewrite <- fold_eps_leaf with (is_bst := is_bst); reflexivity).
-    intro. unfold R.find, R.Raw.find in H. simpl in H. contradict H. reflexivity.
-  - inversion is_bst; subst. 
-    replace (fold_subst_eps
-               {| R.this := R.Raw.Node this1 k e this2 t; R.is_bst := is_bst |} e')
-    with (fold_subst_eps {| R.this := this2; R.is_bst := H6 |}
-                         (subst_eps k (Rgn_Const true false e)
-                                    (fold_subst_eps {| R.this := this1; R.is_bst := H4 |} e')))
-    by (rewrite <- fold_eps_node with (Hr:=H6) (Hl:=H4); reflexivity).
-    intro.
-    (*apply NotNoneIsSome in H. destruct H.
-    eapply decompose_find_in_rho in H.*)
-    destruct (AsciiVars.compare x k); subst.
-    + apply TcRhoIncludedNoFreeVarsEps_aux_fold in H0.
-      apply TcRhoIncludedNoFreeVarsEps in H0. 
-      contradict H0.
-      apply IHthis1.
-      assert (~ R.Raw.In k this1) by (apply RProofs.lt_tree_not_in in H7; auto).
-      assert (~ R.Raw.In k this2) by (apply RProofs.gt_tree_not_in in H8; auto).
-      eapply FindIfLowerThan; eauto.
-    + inversion e0; subst.
-      apply TcRhoIncludedNoFreeVarsEps_aux_fold in H0.
-      contradict H0.
-      apply TcRhoIncludedNoFreeVarsEps_aux.
-    + contradict H0.
-      apply IHthis2.
-      eapply FindIfGreaterThan; eauto.
+  forall (rho: Rho) (x: RgnName),
+    rho !! x <> None ->
+    forall e, ~(free_rgn_vars_in_eps (fold_subst_eps rho e)) x.
+Proof.
+  intros.
+  unfold find_R in H.
+  apply NotNoneIsSome in H. destruct H as [v H].
+  apply find_R_in_list with (p:=(x,v)) in H.
+  rewrite fold_subst_eps_fold_foldr.
+  induction (map_to_list rho); simpl.
+  - contradict H.
+    apply not_elem_of_nil.
+  - rewrite fold_subst_eps_cons.
+    apply not_free_vars_compose_head_eps_fold. 
+    apply elem_of_cons in H.
+    destruct H as [Ha | Hb].
+    + intro. destruct H.
+      subst. clear IHl. clear H0. 
+      unfold free_rgn_vars_in_eps, fold_subst_eps_alt_head in *.
+      destruct H as [sa [[sa' [H1 H2]]]].
+      rewrite <- H2 in H.  clear H2. 
+      contradict H. apply not_free_vars_in_head_after_subst.                
+    + intro. destruct H.
+      apply IHl; assumption.
 Qed.
 
 
@@ -797,15 +1467,17 @@ Proof.
       intros. apply HInc. apply Union_introl. assumption.
     + destruct H0.
       * { destruct H0.
-          - eapply TcRhoIncludedNoFreeVarsEps_main  with (e:=e); eauto.
-            + unfold In in H0. eapply TcRhoIncludedNoFreeVarsEps_aux_fold; eauto. 
+          - eapply TcRhoIncludedNoFreeVarsEps_main  with (e:=e); eauto. 
+            + unfold In in H0. eapply TcRhoIncludedNoFreeVarsEps_aux_fold. 
+              apply free_rgn_vars_in_eps_map_to_list. eauto. 
             + unfold included, Included, Ensembles.In in *.
               intro. intro.
               apply HInc.
               apply Ensembles.Union_intror. apply Ensembles.Union_introl.
               apply Ensembles.Union_introl. assumption.
           - eapply TcRhoIncludedNoFreeVarsEps_main with (e:=e0); eauto.
-            + unfold In in H0. eapply TcRhoIncludedNoFreeVarsEps_aux_fold; eauto. 
+            + unfold In in H0. eapply TcRhoIncludedNoFreeVarsEps_aux_fold.
+              apply free_rgn_vars_in_eps_map_to_list. eauto. 
             + unfold included, Included, Ensembles.In in *.
               intro. intro. apply HInc.
               apply Ensembles.Union_intror. apply Ensembles.Union_introl.
@@ -823,7 +1495,8 @@ Proof.
     unfold not_set_elem, Complement. intro.
     destruct H0.
     + eapply TcRhoIncludedNoFreeVarsEps_main with (e:=e); eauto. 
-      * eapply TcRhoIncludedNoFreeVarsEps_aux_fold; eauto. 
+      * eapply TcRhoIncludedNoFreeVarsEps_aux_fold.
+        apply free_rgn_vars_in_eps_map_to_list. eauto. 
       * unfold included, Included, In in *. intro. intro.
         apply HInc.
         apply Union_introl. assumption.
@@ -834,67 +1507,8 @@ Proof.
 Qed.
 
 
-
-
-Lemma subst_rho_free_vars_rgn_aux_1:
-  forall this1 this2 k e t Hc Hl x r,
-    R.find (elt:=nat) x {| R.this := R.Raw.Node this1 k e this2 t; R.is_bst := Hc |} =
-     None ->
-    free_rgn_vars_in_rgn (fold_subst_rgn {| R.this := this1; R.is_bst := Hl |} r) x ->
-    fold_subst_rgn {| R.this := R.Raw.Node this1 k e this2 t; R.is_bst := Hc |} r = 
-    fold_subst_rgn {| R.this := this1; R.is_bst := Hl |} r.
-Proof.
-  intros. unfold Region_in_Type in r. dependent induction r; 
-  eapply TcRhoIncludedNoFreeVarsRgn_aux_fold in H0; eauto.
-  + unfold free_rgn_vars_in_rgn in *; simpl in *. 
-    inversion H0.
-  + symmetry. rewrite fold_subst_rho_free_vars_rgn_aux. 
-    symmetry. rewrite fold_subst_rho_free_vars_rgn_aux.
-    reflexivity.
-    * simpl in H0. inversion H0. subst.
-      assumption.
-    * simpl in H0. inversion H0. subst.
-      apply RMapP.not_find_in_iff in H. 
-      inversion Hc; subst.
-      eapply not_in_raw_rho with (Hr:=H7) in H; auto.
-      destruct H as [HNotIn1 [HNotIn2 [HNotIn3  HNotIn4]]]. 
-      apply RMapP.not_find_in_iff.
-      eassumption.
-  + unfold free_rgn_vars_in_rgn in *; simpl in *. 
-    inversion H0.
-Qed.
-
-Lemma subst_rho_free_vars_rgn_aux_2:
-  forall this1 this2 k e t Hc Hr x r,
-    R.find (elt:=nat) x {| R.this := R.Raw.Node this1 k e this2 t; R.is_bst := Hc |} =
-     None ->
-    free_rgn_vars_in_rgn (fold_subst_rgn {| R.this := this2; R.is_bst := Hr |} r) x ->
-    fold_subst_rgn {| R.this := R.Raw.Node this1 k e this2 t; R.is_bst := Hc |} r = 
-    fold_subst_rgn {| R.this := this2; R.is_bst := Hr |} r.
-Proof.
-  intros. unfold Region_in_Type in r. dependent induction r; 
-  eapply TcRhoIncludedNoFreeVarsRgn_aux_fold in H0; eauto.
-  + unfold free_rgn_vars_in_rgn in *; simpl in *. 
-    inversion H0.
-  + symmetry. rewrite fold_subst_rho_free_vars_rgn_aux. 
-    symmetry. rewrite fold_subst_rho_free_vars_rgn_aux.
-    reflexivity.
-    * simpl in H0. inversion H0. subst.
-      assumption.
-    * simpl in H0. inversion H0. subst.
-      apply RMapP.not_find_in_iff in H. 
-      inversion Hc; subst.
-      eapply not_in_raw_rho with (Hl:=H5) in H; auto.
-      destruct H as [HNotIn1 [HNotIn2 [HNotIn3  HNotIn4]]]. 
-      apply RMapP.not_find_in_iff.
-      eassumption.
-  + unfold free_rgn_vars_in_rgn in *; simpl in *. 
-    inversion H0.
-Qed.
-
-
 Lemma subst_rho_free_vars_union_1 :
-  forall x (e1 e2 : Ensemble VarId),
+  forall x (e1 e2 : Ensemble RgnName),
     not_set_elem (set_union e1 e2) x ->
     not_set_elem e1 x /\ not_set_elem e2 x.
 Proof.
@@ -902,183 +1516,29 @@ Proof.
 Qed.
 
 Lemma subst_rho_free_vars_union_2 :
-  forall x (e1 e2 : Ensemble VarId),
+  forall x (e1 e2 : Ensemble RgnName),
     not_set_elem e1 x /\ not_set_elem e2 x ->
     not_set_elem (set_union e1 e2) x.
 Proof.
   intros. destruct H. intro. destruct H1; [apply H | apply H0]; auto.
 Qed.
 
-Lemma subst_rho_free_vars_sa_aux_1:
-  forall this1 this2 k e t Hc Hl x sa,
-    R.find (elt:=nat) x {| R.this := R.Raw.Node this1 k e this2 t; R.is_bst := Hc |} =
-     None ->
-    free_rgn_vars_in_sa (fold_subst_sa {| R.this := this1; R.is_bst := Hl |} sa) x ->
-    fold_subst_sa {| R.this := R.Raw.Node this1 k e this2 t; R.is_bst := Hc |} sa = 
-    fold_subst_sa {| R.this := this1; R.is_bst := Hl |} sa.
-Proof.
-  intros. induction sa;
-  unfold free_rgn_vars_in_sa in *; simpl in *; f_equal;
-  eapply subst_rho_free_vars_rgn_aux_1; eauto.
-Qed.
-
-Lemma subst_rho_free_vars_sa_aux_2:
-  forall this1 this2 k e t Hc Hr x sa,
-    R.find (elt:=nat) x {| R.this := R.Raw.Node this1 k e this2 t; R.is_bst := Hc |} =
-     None ->
-    free_rgn_vars_in_sa (fold_subst_sa {| R.this := this2; R.is_bst := Hr |} sa) x ->
-    fold_subst_sa {| R.this := R.Raw.Node this1 k e this2 t; R.is_bst := Hc |} sa = 
-    fold_subst_sa {| R.this := this2; R.is_bst := Hr |} sa.
-Proof.
-  intros. induction sa;
-  unfold free_rgn_vars_in_sa in *; simpl in *; f_equal;
-  eapply subst_rho_free_vars_rgn_aux_2; eauto.
-Qed.
-
-
-Lemma subst_rho_free_vars_eps_aux_1:
-  forall this1 this2 k e t Hc Hl x e',
-    R.find (elt:=nat) x {| R.this := R.Raw.Node this1 k e this2 t; R.is_bst := Hc |} =
-     None ->
-   free_rgn_vars_in_eps (fold_subst_eps {| R.this := this1; R.is_bst := Hl |} e') x ->
-   free_rgn_vars_in_eps (fold_subst_eps
-                     {| R.this := R.Raw.Node this1 k e this2 t; R.is_bst := Hc |} e') x.
-Proof.
-  intros. 
-  unfold fold_subst_eps in *.
-  destruct H0 as [sa1 [[sa1' [H1a H1b]] H1c]].
-  exists sa1. split; [| assumption].
-  exists sa1'. split; [assumption |].
-  rewrite <- H1b.
-  rewrite <- H1b in H1c.
-  eapply subst_rho_free_vars_sa_aux_1; eauto.
-Qed.
-
-
-Lemma subst_rho_free_vars_eps_aux_2:
-  forall this1 this2 k e t Hc Hr x e',
-    R.find (elt:=nat) x {| R.this := R.Raw.Node this1 k e this2 t; R.is_bst := Hc |} =
-     None ->
-    free_rgn_vars_in_eps (fold_subst_eps {| R.this := this2; R.is_bst := Hr |} e') x ->
-    free_rgn_vars_in_eps (fold_subst_eps
-                     {| R.this := R.Raw.Node this1 k e this2 t; R.is_bst := Hc |} e') x.
-Proof.
-  intros. 
-  unfold fold_subst_eps in *.
-  destruct H0 as [sa1 [[sa1' [H1a H1b]] H1c]].
-  exists sa1. split; [| assumption].
-  exists sa1'. split; [assumption |].
-  rewrite <- H1b.
-  rewrite <- H1b in H1c.
-  eapply subst_rho_free_vars_sa_aux_2; eauto.
-Qed.
-
-Lemma equal_fold_subst_rgn:
-  forall this1 this2 k e t Hc r,
-    R.find (elt:=nat) k {| R.this := R.Raw.Node this1 k e this2 t; R.is_bst := Hc |} = None ->
-    free_rgn_vars_in_rgn r k ->
-    fold_subst_rgn {| R.this := R.Raw.Node this1 k e this2 t; R.is_bst := Hc |} r = r.
-Proof.
-  intros. unfold Region_in_Type in r. dependent induction r; simpl in *.
-  - inversion H0.
-  - inversion H0. subst.
-    apply fold_subst_rho_free_vars_rgn_aux. auto.   
-  - inversion H0.
-Qed.
-
-Lemma equal_fold_subst_sa:
-  forall this1 this2 k e t Hc sa, 
-    R.find (elt:=nat) k {| R.this := R.Raw.Node this1 k e this2 t; R.is_bst := Hc |} = None ->
-    free_rgn_vars_in_sa sa k ->
-    fold_subst_sa {| R.this := R.Raw.Node this1 k e this2 t; R.is_bst := Hc |} sa = sa.
-Proof.
-  intros. induction sa; simpl in *; f_equal; apply equal_fold_subst_rgn; auto.
-Qed.
-
-
-Lemma baz:
-  forall (rho : R.t RgnId),
-  forall (k': R.key) (v': RgnId),
-    ~ R.In k' rho ->
-    exists elems1 elems2,
-      elems1 ++ (k',v')::elems2 = R.elements (R.add k' v' rho) /\
-      elems1 ++ elems2 = R.elements rho.
-Proof.
-  destruct rho. induction this; intros k' v' H.
-  - exists nil. exists nil. intuition.
-  - destruct (AsciiVars.compare k' k).
-    + admit.
-    + inversion e0; subst.
-      contradict H. unfold R.In, R.Raw.In0. simpl. eauto.
-    + admit.
-Admitted.
-
-Lemma fold_subst:
-  forall A,
-  forall (f : A -> (R.key * RgnId) -> A),
-  forall l1 x' l2 b,
-    (forall (y : R.key * RgnId) b0,
-       In y l1 ->
-       f (f b0 y) x' = f (f b0 x') y) ->
-    List.fold_left f (l1 ++ x'::l2) b = fold_left f (l1 ++ l2) (f b x'). 
-Proof.  
-  intros f. 
-  induction l1; intros x' l2 b H. 
-  - simpl. reflexivity.
-  - simpl. rewrite IHl1.
-    + rewrite H.
-      * reflexivity.
-      * apply in_eq.
-    + intros y b0 In_y. apply H. apply in_cons. apply In_y.
-Qed.
-
-
-Lemma fold_add_type:
-  forall A,
-  forall (f : R.key -> RgnId -> A -> A),
-  forall (rho : R.t RgnId),
-  forall (k': R.key) (v': RgnId) (b: A),
-    ~ R.In k' rho ->
-    (forall k v b0,
-       R.MapsTo k v rho ->
-       f k' v' (f k v b0) = f k v (f k' v' b0)) ->
-    R.fold f (R.add k' v' rho) b = R.fold f rho (f k' v' b).
-Proof.
-  intros A f rho k' v' b H' H.
-  repeat (rewrite R.fold_1). 
-  destruct (baz rho k' v' H') as [elems1 [elems2 [H1 H2]]]. 
-  rewrite <- H1.
-  rewrite <- H2.
-  apply fold_subst.
-  intros [k1 v1] b0 In_k1_v1. simpl. apply H.
-  apply R.elements_2.
-  apply In_InA.
-  - repeat constructor.
-    + destruct H0. auto.
-    + destruct H0; auto.
-    + destruct H0; rewrite H0. destruct H3. auto.
-    + destruct H0; rewrite H4. destruct H3. auto.
-  - rewrite <- H2.
-    apply List.in_or_app. left. apply In_k1_v1.
-Qed.
 
 
 Lemma contrapositiveTcRho :
-  forall rho rgns x,
-    (forall r : R.key, 
-       R.find (elt:=nat) r rho <> None -> set_elem rgns r) ->
+  forall (rho : Rho) (rgns : Ensemble RgnName) (x : RgnName),
+    (forall r, rho !! r <> None -> set_elem rgns r) ->
     not_set_elem rgns x ->
-    R.find (elt:=nat) x rho = None.
+    rho !! x = None.
 Proof.
   intros.
   unfold not_set_elem in H0. unfold Ensembles.Complement in H0.
-  unfold set_elem in H. unfold Ensembles.Complement in H.
-  apply RMapP.not_find_in_iff.
+  unfold set_elem in H. unfold Ensembles.Complement in H. 
+  apply not_elem_of_dom.
   intro. apply H0.
+  assert (Hr : forall r (rho : Rho), r ∈ dom rho -> rho !! r <> None)
+    by (intros; apply elem_of_dom in H2; apply not_eq_None_Some in H2; assumption).
   apply H.
-  assert (Hr : forall t r rho,
-             R.In (elt:=t) r rho -> R.find (elt:=t) r rho <> None) by
-    (intros; apply RMapP.in_find_iff; auto).
   apply Hr.
   assumption.
 Qed.
